\documentclass[12pt]{article}
\usepackage{amsmath}
\usepackage{amsfonts}
\usepackage{geometry}
\geometry{margin=1in}

\title{Limits exercise}
\author{}
\date{}

\begin{document}

\maketitle

\section*{Problem 1: Evaluate the following limits}

\subsection*{(i) \(\displaystyle \lim_{x \to 1} \frac{x^2 - 1}{x + 1}\)}

\textbf{Algebraic Approach:}
\[
\frac{x^2 - 1}{x + 1} = \frac{(x - 1)(x + 1)}{x + 1} = x - 1
\]
\[
\lim_{x \to 1} (x - 1) = 0
\]

\textbf{L'Hôpital's Rule:}
\[
\lim_{x \to 1} \frac{x^2 - 1}{x + 1} = \frac{0}{2} = 0 \quad \text{(Direct substitution, no 0/0)}
\]

\textbf{Answer:} \(\boxed{0}\)

\subsection*{(ii) \(\displaystyle \lim_{x \to 2} \frac{x^3 - 8}{x - 2}\)}

\textbf{Algebraic Approach:}
\[
x^3 - 8 = (x - 2)(x^2 + 2x + 4)
\]
\[
\frac{x^3 - 8}{x - 2} = x^2 + 2x + 4
\]
\[
\lim_{x \to 2} x^2 + 2x + 4 = 4 + 4 + 4 = 12
\]

\textbf{L'Hôpital's Rule:}
\[
\lim_{x \to 2} \frac{x^3 - 8}{x - 2} = \lim_{x \to 2} \frac{3x^2}{1} = 3 \cdot 4 = 12
\]

\textbf{Answer:} \(\boxed{12}\)

\subsection*{(iii) \(\displaystyle \lim_{x \to 3} \frac{x^3 - 8}{x - 2}\)}

\textbf{Direct Substitution:}
\[
\frac{27 - 8}{3 - 2} = \frac{19}{1} = 19
\]

\textbf{Answer:} \(\boxed{19}\)

\subsection*{(iv) \(\displaystyle \lim_{x \to y} \frac{x^n - y^n}{x - y}\)}

\textbf{Algebraic Identity:}
\[
\frac{x^n - y^n}{x - y} = \sum_{k=0}^{n-1} x^{n-1-k} y^k
\Rightarrow \lim_{x \to y} \sum_{k=0}^{n-1} x^{n-1-k} y^k = n y^{n-1}
\]

\textbf{L’Hôpital’s Rule:}
\[
\lim_{x \to y} \frac{d}{dx} \left( x^n \right) = \frac{n x^{n-1}}{1} \Rightarrow \text{at } x = y: \quad n y^{n-1}
\]

\textbf{Answer:} \(\boxed{n y^{n-1}}\)

\subsection*{(v) \(\displaystyle \lim_{y \to x} \frac{x^n - y^n}{x - y}\)}

This is symmetric to (iv), with \(x\) and \(y\) switched.

\textbf{Using symmetry:}
\[
\lim_{y \to x} \frac{x^n - y^n}{x - y} = \lim_{y \to x} \frac{y^n - x^n}{y - x} = n x^{n-1}
\]

\textbf{L’Hôpital’s Rule:}
\[
\frac{d}{dy}(-y^n) = -n y^{n-1} \Rightarrow \text{At } y = x: \quad n x^{n-1}
\]

\textbf{Answer:} \(\boxed{n x^{n-1}}\)

\subsection*{(vi) \(\displaystyle \lim_{h \to 0} \frac{\sqrt{a + h} - \sqrt{a}}{h}\)}

\textbf{Multiply numerator and denominator by the conjugate:}
\[
\frac{\sqrt{a + h} - \sqrt{a}}{h} \cdot \frac{\sqrt{a + h} + \sqrt{a}}{\sqrt{a + h} + \sqrt{a}} =
\frac{(a + h) - a}{h(\sqrt{a + h} + \sqrt{a})} = \frac{1}{\sqrt{a + h} + \sqrt{a}}
\]
\[
\lim_{h \to 0} \frac{1}{\sqrt{a + h} + \sqrt{a}} = \frac{1}{2 \sqrt{a}}
\]

\textbf{L’Hôpital’s Rule:}
\[
\frac{d}{dh} \left( \sqrt{a + h} \right) = \frac{1}{2 \sqrt{a + h}} \Rightarrow \text{At } h = 0: \frac{1}{2 \sqrt{a}}
\]

\textbf{Answer:} \(\boxed{\dfrac{1}{2 \sqrt{a}}}\)

\end{document}
